src/lowparse/LowParse.SLow.VLData.Header.fst
@@ -1,0 +1,53 @@
+module LowParse.SLow.VLData.Header
+
+friend LowParse.Spec.VLData.Header
+
+module Seq = FStar.Seq
+module U32 = FStar.UInt32
+module E = LowParse.BigEndianImpl.SLow
+module B32 = LowParse.Bytes32
+
+let serialize32_bounded_integer_1
+= (fun (input: bounded_integer 1) ->
+    let b = E.n_to_be_1 _ _ (E.u32 ()) input in
+    (b <: (res: B32.bytes { serializer32_correct (serialize_bounded_integer 1) input res } ))
+  )
+
+let serialize32_bounded_integer_2
+= (fun (input: bounded_integer 2) ->
+    let b = E.n_to_be_2 _ _ (E.u32 ()) input in
+    (b <: (res: B32.bytes { serializer32_correct (serialize_bounded_integer 2) input res } ))
+  )
+
+let serialize32_bounded_integer_3
+= (fun (input: bounded_integer 3) ->
+    let b = E.n_to_be_3 _ _ (E.u32 ()) input in
+    (b <: (res: B32.bytes { serializer32_correct (serialize_bounded_integer 3) input res } ))
+  )
+
+let serialize32_bounded_integer_4
+= (fun (input: bounded_integer 4) ->
+    let b = E.n_to_be_4 _ _ (E.u32 ()) input in
+    (b <: (res: B32.bytes { serializer32_correct (serialize_bounded_integer 4) input res } ))
+  )
+
+let decode32_bounded_integer_1 b
+= let r = E.be_to_n_1 _ _ (E.u32 ()) b in
+  E.lemma_be_to_n_is_bounded (B32.reveal b);
+  (r <: (r: bounded_integer 1 { r == decode_bounded_integer 1 (B32.reveal b) } ))
+
+let decode32_bounded_integer_2 b
+= let r = E.be_to_n_2 _ _ (E.u32 ()) b in
+  E.lemma_be_to_n_is_bounded (B32.reveal b);
+  (r <: (r: bounded_integer 2 { r == decode_bounded_integer 2 (B32.reveal b) } ))
+
+let decode32_bounded_integer_3 b
+= let r = E.be_to_n_3 _ _ (E.u32 ()) b in
+  E.lemma_be_to_n_is_bounded (B32.reveal b);
+  (r <: (r: bounded_integer 3 { r == decode_bounded_integer 3 (B32.reveal b) } ))
+
+let decode32_bounded_integer_4 b
+= let r = E.be_to_n_4 _ _ (E.u32 ()) b in
+  E.lemma_be_to_n_is_bounded (B32.reveal b);
+  (r <: (r: bounded_integer 4 { r == decode_bounded_integer 4 (B32.reveal b) } ))
+
