src/lowparse/LowParse.SLow.VLData.Header.fsti
@@ -1,0 +1,66 @@
+module LowParse.SLow.VLData.Header
+include LowParse.Spec.VLData.Header
+include LowParse.SLow.Combinators
+
+module Seq = FStar.Seq
+module U32 = FStar.UInt32
+module B32 = LowParse.Bytes32
+
+val serialize32_bounded_integer_1
+: (serializer32 (serialize_bounded_integer 1))
+
+val serialize32_bounded_integer_2
+: (serializer32 (serialize_bounded_integer 2))
+
+val serialize32_bounded_integer_3
+: (serializer32 (serialize_bounded_integer 3))
+
+val serialize32_bounded_integer_4
+: (serializer32 (serialize_bounded_integer 4))
+
+inline_for_extraction
+let serialize32_bounded_integer
+  (sz: integer_size)
+: Tot (serializer32 (serialize_bounded_integer sz))
+= match sz with
+  | 1 -> serialize32_bounded_integer_1
+  | 2 -> serialize32_bounded_integer_2
+  | 3 -> serialize32_bounded_integer_3
+  | 4 -> serialize32_bounded_integer_4
+
+val decode32_bounded_integer_1
+  (b: B32.lbytes 1)
+: Tot (y: bounded_integer 1 { y == decode_bounded_integer 1 (B32.reveal b) } )
+
+val decode32_bounded_integer_2
+  (b: B32.lbytes 2)
+: Tot (y: bounded_integer 2 { y == decode_bounded_integer 2 (B32.reveal b) } )
+
+val decode32_bounded_integer_3
+  (b: B32.lbytes 3)
+: Tot (y: bounded_integer 3 { y == decode_bounded_integer 3 (B32.reveal b) } )
+
+val decode32_bounded_integer_4
+  (b: B32.lbytes 4)
+: Tot (y: bounded_integer 4 { y == decode_bounded_integer 4 (B32.reveal b) } )
+
+inline_for_extraction
+let decode32_bounded_integer
+  (sz: integer_size)
+: Tot ((b: B32.lbytes sz) ->
+    Tot (y: bounded_integer sz { y == decode_bounded_integer sz (B32.reveal b) } )
+  )
+= match sz with
+  | 1 -> decode32_bounded_integer_1
+  | 2 -> decode32_bounded_integer_2
+  | 3 -> decode32_bounded_integer_3
+  | 4 -> decode32_bounded_integer_4
+
+inline_for_extraction
+let parse32_bounded_integer (sz: integer_size) : Tot (parser32 (parse_bounded_integer sz)) =
+  [@inline_let]
+  let _ = decode_bounded_integer_injective sz in
+  make_total_constant_size_parser32 sz (U32.uint_to_t sz)
+    (decode_bounded_integer sz)
+    ()
+    (decode32_bounded_integer sz)
