src/lowparse/LowParse.Spec.VLData.Header.fst
@@ -1,0 +1,63 @@
+module LowParse.Spec.VLData.Header
+
+module U32 = FStar.UInt32
+module E = LowParse.BigEndian
+
+#reset-options "--z3cliopt smt.arith.nl=false --using_facts_from '*  -FStar.UInt8 -FStar.UInt16' --z3rlimit 32"
+
+let integer_size_values i = ()
+
+#reset-options
+
+let decode_bounded_integer i b
+= E.lemma_be_to_n_is_bounded b;
+  U32.uint_to_t (E.be_to_n b)
+
+#set-options "--z3rlimit 16"
+let decode_bounded_integer_injective'
+  (i: integer_size)
+  (b1: bytes { Seq.length b1 == i } )
+  (b2: bytes { Seq.length b2 == i } )
+: Lemma
+  (decode_bounded_integer i b1 == decode_bounded_integer i b2 ==> Seq.equal b1 b2)
+= if decode_bounded_integer i b1 = decode_bounded_integer i b2
+  then begin
+    E.lemma_be_to_n_is_bounded b1;
+    E.lemma_be_to_n_is_bounded b2;
+    assert (U32.v (U32.uint_to_t (E.be_to_n b1)) == E.be_to_n b1);
+    assert (U32.v (U32.uint_to_t (E.be_to_n b2)) == E.be_to_n b2);
+    assert (E.be_to_n b1 == E.be_to_n b2);
+    E.be_to_n_inj b1 b2
+  end else ()
+#reset-options
+
+let decode_bounded_integer_injective i
+= Classical.forall_intro_2 (decode_bounded_integer_injective' i)
+
+let serialize_bounded_integer'
+  (sz: integer_size)
+: Tot (bare_serializer (bounded_integer sz))
+= (fun (x: bounded_integer sz) ->
+    let res = E.n_to_be (U32.uint_to_t sz) (U32.v x) in
+    res
+  )
+
+let serialize_bounded_integer_correct
+  (sz: integer_size)
+: Lemma
+  (serializer_correct (parse_bounded_integer sz) (serialize_bounded_integer' sz))
+= let prf
+    (x: bounded_integer sz)
+  : Lemma
+    (
+      let res = serialize_bounded_integer' sz x in
+      Seq.length res == (sz <: nat) /\
+      parse (parse_bounded_integer sz) res == Some (x, (sz <: nat))
+    )
+  = ()
+  in
+  Classical.forall_intro prf
+
+let serialize_bounded_integer sz
+= serialize_bounded_integer_correct sz;
+  serialize_bounded_integer' sz
