src/lowparse/LowParse.Spec.VLData.Header.fsti
@@ -1,0 +1,41 @@
+module LowParse.Spec.VLData.Header
+include LowParse.Spec.Combinators
+
+module U32 = FStar.UInt32
+
+let integer_size : Type0 = (sz: nat { 1 <= sz /\ sz <= 4 } )
+
+val integer_size_values (i: integer_size) : Lemma
+  (i == 1 \/ i == 2 \/ i == 3 \/ i == 4)
+
+inline_for_extraction
+let bounded_integer
+  (i: integer_size)
+: Tot Type0
+= (u: U32.t { U32.v u < pow2 (FStar.Mul.op_Star 8 i) } )
+
+val decode_bounded_integer
+  (i: integer_size)
+  (b: bytes { Seq.length b == i } )
+: GTot (bounded_integer i)
+
+val decode_bounded_integer_injective
+  (i: integer_size)
+: Lemma
+  (make_total_constant_size_parser_precond i (bounded_integer i) (decode_bounded_integer i))
+
+// unfold
+let parse_bounded_integer_kind
+  (i: integer_size)
+: Tot parser_kind
+= total_constant_size_parser_kind i
+
+let parse_bounded_integer
+  (i: integer_size)
+: Tot (parser (parse_bounded_integer_kind i) (bounded_integer i))
+= decode_bounded_integer_injective i;
+  make_total_constant_size_parser i (bounded_integer i) (decode_bounded_integer i)
+
+val serialize_bounded_integer
+  (sz: integer_size)
+: Tot (serializer (parse_bounded_integer sz))
